# Arithmetics

$$
a^n-b^n=(a-b)(a^{n-1}+a^{n-2}b+\cdots+ab^{n-2}+b^{n-1})
$$

$$
\log xy=\log x+\log y
\\
\log x^r=r\log x
$$

$$
\frac{\sqrt{a^2+b^2}-b}{a^2}
=\frac{a^2}{\sqrt{a^2+b^2}+b}
$$

sigma notation

$$
\sum_{i=m}^nf(x_i)
$$

- linear

common sum

$$
\sum_{i=1}^ni=\frac{n(n+1)}{2}
\\[12pt]
\sum_{i=1}^ni^2=\frac{n(n+1)(2n+1)}{6}
\\[12pt]
\sum_{i=1}^ni^3=\left[
    \frac{n(n+1)}{2}
\right]^2
$$

trigonometric transformation

$$
\sin A\cos B
=\frac{1}{2}[\sin(A-B)+\sin(A+B)]
\\[12pt]
\sin A\sin B
=\frac{1}{2}[\cos(A-B)-\cos(A+B)]
\\[12pt]
\cos A\cos B
=\frac{1}{2}[\cos(A-B)+\cos(A+B)]
$$
